proofs/transform/eliminate_algebraic_proofs.v
@@ -138,6 +138,225 @@ Proof.
   unfold trans_pre_post, task_and. intros; split; eauto.
 Qed.
 
+(*Interlude: Reason about inhabited types if we remove some ADTs*)
+
+(*Mutual ADTs are subset of another*)
+Definition mut_adt_subset (m1 m2: mut_adt) : Prop :=
+  (m_params m1) = (m_params m2) /\
+  sublist (typs m1) (typs m2) .
+
+Fixpoint mut_adts_subset (l1 l2: list mut_adt) : Prop :=
+  match l1, l2 with
+  | nil, _ => True
+  | m1 :: t1, m2 :: t2 => (mut_adt_subset m1 m2 /\ mut_adts_subset t1 t2) \/
+    (mut_adts_subset (m1 :: t1) t2)
+  | _ :: _, nil => False
+  end.
+
+(*TODO: should generalize*)
+Definition find_ts_in_ctx_gen (l: list mut_adt) (ts: typesym) :=
+  fold_right (fun m acc => 
+    match (find_ts_in_mut ts m) with
+    | Some a => Some (m, a)
+    | None => acc
+    end) None l.
+
+Lemma find_ts_in_ctx_gen_eq (gamma: context) (ts: typesym) :
+  find_ts_in_ctx gamma ts = find_ts_in_ctx_gen (mut_of_context gamma) ts.
+Proof. reflexivity. Qed.
+
+Lemma find_ts_in_mut_in (m: mut_adt) (ts: typesym) x:
+  find_ts_in_mut ts m = Some x ->
+  In ts (typesyms_of_mut m).
+Proof.
+  intros Hfind. apply find_ts_in_mut_some in Hfind.
+  unfold typesyms_of_mut. destruct Hfind as [a_in Hts]; subst.
+  rewrite in_map_iff. exists x; split; auto. apply in_bool_In in a_in; auto.
+Qed.
+
+Lemma find_ts_in_ctx_gen_in (l: list mut_adt) (ts: typesym) x :
+  find_ts_in_ctx_gen l ts = Some x ->
+  In ts (concat (map typesyms_of_mut l)).
+Proof.
+  induction l as [| m1 t1 IH]; simpl; auto; [discriminate|].
+  destruct (find_ts_in_mut ts m1) as [a1|] eqn : Hfind.
+  - inv Hsome. rewrite in_app_iff; left.
+    apply find_ts_in_mut_in in Hfind; auto.
+  - intros Hfind1. rewrite in_app_iff; right; auto.
+Qed.
+
+Lemma find_sublist {A: Type} (l1 l2: list A) (p: A -> bool) x:
+  sublist l1 l2 ->
+  (forall x y, In x l2 -> In y l2 -> p x -> p y -> x = y) ->
+  find p l1 = Some x ->
+  find p l2 = Some x.
+Proof.
+  intros Hsub Heq Hfind. apply find_some in Hfind. rewrite find_some_nodup; auto.
+  destruct Hfind as [Hin Hp]. split; auto.
+Qed.
+
+(*We do need some info about uniqueness of names, should be OK*)
+
+(*Condition for uniqueness of ADT names*)
+Definition adts_uniq (l: list mut_adt) : Prop :=
+  NoDup (concat (map typesyms_of_mut l)).
+
+
+Lemma mut_adt_subset_typesyms (m1 m2: mut_adt):
+  mut_adt_subset m1 m2 ->
+  sublist (typesyms_of_mut m1) (typesyms_of_mut m2).
+Proof.
+  unfold mut_adt_subset, typesyms_of_mut.
+  intros [_ Hsub]. apply sublist_map; auto.
+Qed.
+
+(*A crucial part as to why our subset criterion is correct*)
+Lemma mut_adts_subset_typesyms (l1 l2: list mut_adt):
+  mut_adts_subset l1 l2 ->
+  sublist (concat (map typesyms_of_mut l1)) (concat (map typesyms_of_mut l2)).
+Proof.
+  revert l1. induction l2 as [| m2 t2 IH]; intros [|m1 t1]; simpl; auto; try contradiction.
+  - intros _; apply sublist_nil_l.
+  - intros _; apply sublist_nil_l.
+  - intros [[Hm12 Hsub] | Hsub].
+    + apply sublist_app2; auto. 
+      apply mut_adt_subset_typesyms; auto.
+    + eapply sublist_trans; [| apply sublist_app_r].
+      apply (IH _ Hsub).
+Qed.
+
+(*The main structural result we need: looking up the type in the smaller set
+  gives the same ADT as in the larger set*)
+Lemma mut_adts_subset_find_ts (l1 l2: list mut_adt):
+  mut_adts_subset l1 l2 ->
+  adts_uniq l2 ->
+  forall ts m1 a, find_ts_in_ctx_gen l1 ts = Some (m1, a) ->
+    exists (m2: mut_adt), find_ts_in_ctx_gen l2 ts = Some (m2,  a) /\
+    mut_adt_subset m1 m2.
+Proof.
+  revert l1. induction l2 as [| m2 t2 IH]; intros [| m1 t1]; simpl; auto; 
+  try discriminate; try contradiction.
+  intros [[Hm12 Hsub] | Hsub] Huniq.
+  - intros ts m3 a. destruct (find_ts_in_mut ts m1) as [a1|] eqn : Hfind.
+    + inv Hsome. exists m2.
+      unfold find_ts_in_mut in Hfind |- *.
+      apply find_sublist with (l2:=typs m2) in Hfind ; [| apply Hm12 |].
+      * rewrite Hfind. auto.
+      * (*From NoDups, get uniquness condition*)
+        unfold adts_uniq in Huniq. simpl in Huniq. rewrite NoDup_app_iff in Huniq.
+        destruct Huniq as [Huniq _]. unfold typesyms_of_mut in Huniq.
+        intros x y Hinx Hiny. do 2 (destruct (typesym_eq_dec _ _); try discriminate).
+        intros _ _. subst. apply (@NoDup_map_in _ _ _ _ x y) in Huniq; auto.
+    + intros Hfind1.
+      destruct (find_ts_in_mut ts m2) as [a2|] eqn : Hfind2.
+      * (*Idea: contradiction: this typesym cannot appear in later list, which it must
+          from [find_ts_in_mut] but cannot from NoDup (it is m2 from find, it is t2 from t1 and subset)*)
+        assert (Hin1: In ts (typesyms_of_mut m2)). {
+          apply find_ts_in_mut_in in Hfind2; auto.
+        }
+        assert (Hin2: In ts (concat (map typesyms_of_mut t2))). {
+          apply find_ts_in_ctx_gen_in in Hfind1.
+          eapply mut_adts_subset_typesyms. apply Hsub. auto.
+        }
+        (*Now contradicts NoDups*)
+        unfold adts_uniq in Huniq.
+        simpl in Huniq. rewrite NoDup_app_iff in Huniq.
+        destruct Huniq as [_ [_ [Hnotin _]]].
+        exfalso. apply (Hnotin _ Hin1 Hin2).
+      * apply (IH t1); auto.
+        unfold adts_uniq in Huniq |- *. simpl in Huniq.
+        apply NoDup_app_iff in Huniq. apply Huniq.
+  - (*Other case, skip m2*)
+    intros ts m3 a. 
+    specialize (IH _ Hsub).
+    simpl in IH.
+    forward IH.
+    {
+      unfold adts_uniq in Huniq |- *. simpl in Huniq.
+      rewrite NoDup_app_iff in Huniq; apply Huniq.
+    }
+    intros Hfind.
+    (* assert (Hfind2:=Hfind). *)
+    apply IH in Hfind.
+    (*Just need to prove that ts not in m2*)
+    destruct (find_ts_in_mut ts m2) as [a2|] eqn : Hfind3; auto.
+    exfalso.
+    unfold adts_uniq in Huniq; simpl in Huniq.
+    rewrite NoDup_app_iff in Huniq. 
+    destruct Huniq as [_ [_ [Hnotin _]]]; apply (Hnotin ts).
+    + apply find_ts_in_mut_in in Hfind3; assumption.
+    + destruct Hfind as [m4 [Hfind Hsub1]].
+      apply find_ts_in_ctx_gen_in in Hfind; auto.
+Qed.
+
+(*This is a stronger version of [typesym_inhab_fun_sublist]
+  because it does not require the list of mutual types to be the same.
+  Instead, it must be the case that
+  1. All ADTs in g1 are a subset of those in g2
+  2. All ADTs in g2 but not in g1 are still present as abstract symbols
+  3. All ADTs in g2 have unique names
+  This has the other direction as the other lemma because we are "shrinking"
+  a context instead of expanding it*)
+Lemma typesym_inhab_fun_sublist g1 g2 seen ts:
+  mut_adts_subset (mut_of_context g1) (mut_of_context g2) ->
+  sig_t g1 = sig_t g2 -> (*Permutation or equal?*)
+  adts_uniq (mut_of_context g2) ->
+  typesym_inhab_fun g2 seen ts (length (sig_t g1) - length seen) ->
+  typesym_inhab_fun g1 seen ts (length (sig_t g2) - length seen).
+Proof.
+  intros Hmuteq Htseq.
+  rewrite Htseq. remember (length (sig_t g2) - length seen) as n.
+  generalize dependent seen. revert ts.
+  induction n as [| n' IH]; intros ts seen Hlen Huniq Hinhab.
+  - inversion Hinhab.
+  - rewrite typesym_inhab_fun_eq in *.
+    bool_hyps. repeat simpl_sumbool.
+    simpl. bool_to_prop; split_all; auto; try simpl_sumbool.
+    + rewrite <- Htseq in i; contradiction.
+    + destruct (find_ts_in_ctx g1 ts) as [[m1 a1] |] eqn : Hfind; auto.
+      assert (Hfind2:=Hfind).
+      (*Needed all of the above to relate [find_ts_in_ctx] for both*)
+      apply mut_adts_subset_find_ts with (l2:=mut_of_context g2) in Hfind2; auto.
+      destruct Hfind2 as [m2 [Hfind2 Hsub2]].
+      rewrite find_ts_in_ctx_gen_eq in H0. rewrite Hfind2 in H0. 
+      apply andb_true_iff in H0.
+      destruct H0 as [Hnotnull Hex].
+      rewrite Hnotnull. simpl.
+      revert Hex. apply existsb_impl.
+      intros x Hinx.
+      unfold constr_inhab_fun.
+      apply forallb_impl.
+      intros y Hiny.
+      apply vty_inhab_fun_expand.
+      intros ts'. apply IH.
+      simpl. lia. auto.
+Qed.
+(*The above is useful in showing that things are still well-typed even if we do not
+  eliminate certain ADTs in a mutual set*)
+(*End interlude*)
+
+(*The core result: soundness of [fold_comp]
+  TODO: probably need to generalize from [empty_state]*)
+(*We need the precondition that pattern matches have been compiled away*)
+Theorem fold_comp_sound keep_tys noind noinv nosel:
+  sound_trans_pre
+  (task_and no_recfun_indpred task_pat_simpl)
+  (fold_comp keep_tys (empty_state noind noinv nosel)).
+Proof.
+  unfold fold_comp.
+
+  (*remember (fold_left
+(fun (x : state * task) (y : def) =>
+comp_ctx keep_tys y x) (task_gamma t)
+(empty_state noind noinv nosel, t)) as comp.
+  unfold fold_comp. simpl_task.
+
+
+
+  rewrite (surjective_pairing (fold_left _ _ _)).
+  Search fst snd. simpl.*)
+Admitted.
+
 Theorem eliminate_algebraic_sound keep_tys noind noinv nosel : 
   sound_trans_pre no_recfun_indpred
   (eliminate_algebraic keep_tys noind noinv nosel).
